

$$1) Y = a + bX \quad \text{each datapoint: } y_i = a + bx_i$$

$$m(Y) = \frac{1}{N} \sum_{i=1}^N y_i$$

$$M(Y) = \frac{1}{N} \sum_{i=1}^N a + bx_i$$

$$N(M(Y)) = \sum_{i=1}^N a + \sum_{i=1}^N bx_i$$

$$N(M(Y)) = Na + b \sum_{i=1}^N x_i$$

$$M(Y) = \frac{N}{N} a + b \frac{1}{N} \sum_{i=1}^N x_i$$

$$M(Y) = a + bM(X)$$

$$M(a + bX) = a + bM(X)$$

$$2) \text{cov}(X, X) = \frac{1}{N} \sum_{i=1}^N (x_i - m(X))(x_i - m(X))$$

$$\text{cov}(X, X) = \frac{1}{N} \sum_{i=1}^N (x_i - m(X))^2$$

$$\text{cov}(X, X) = s^2$$

$$3) \text{cov}(X, a+bY) = \frac{1}{N} \sum_{i=1}^N (x_i - m(X)) ((a+by_i) - m(a+bY))$$

$$\begin{aligned} \text{cov}(X, a+bY) &= \frac{1}{N} \sum_{i=1}^N (x_i - m(X)) ((a+by_i) - (a+bM(Y))) \\ &= \frac{1}{N} \sum_{i=1}^N (x_i - m(X)) (a+by_i - a - bM(Y)) \\ &= \frac{1}{N} \sum_{i=1}^N (x_i - m(X)) (b(y_i - M(Y))) \\ &= b \left(\frac{1}{N} \sum_{i=1}^N (x_i - m(X)) (y_i - M(Y)) \right) \\ &= b \text{cov}(X, Y) \end{aligned}$$

$$4) \text{cov}(a+bX, a+bY)$$

$$\text{by our proof in \#3: } \text{cov}(a+bX, a+bY) = b \text{cov}(a+bX, Y)$$

$$b \text{cov}(a+bX, Y) = b(b \text{cov}(X, Y))$$

$$\text{cov}(a+bX, a+bY) = b^2 \text{cov}(X, Y)$$

5) Since $b > 0$, order is maintained.

$\text{med}(a+bX)$ = all values are scaled by b , shifted by A , and then the median is taken

$a+b(\text{med}(X))$ = median is taken, and then all values are scaled / shifted.

Because $b > 0$ keeps the order, the middle item (median) remains the middle item through transformations.

$$\text{IQR: } \text{IQR}(X) = Q_3(X) - Q_1(X)$$

$$Y = a + bX \text{ where } b > 0$$

$$Q_1(Y) = a + bQ_1(X), \quad Q_3(Y) = a + bQ_3(X)$$

$$\text{IQR}(Y) = a + bQ_3(X) - a - bQ_1(X)$$

$$\text{IQR}(Y) = b(Q_3(X) - Q_1(X))$$

$$\text{IQR}(Y) = b(\text{IQR}(X))$$

$$\text{IQR}(a + bX) = b(\text{IQR}(X))$$

$$\text{Therefore, } \text{IQR}(a + bX) = a + b(\text{IQR}(X))$$

i) only true when $a = 0$.

6) X^2 :

$$X = \{0, 1, 2\}$$

$$\text{mean of } X^2 = \frac{0 + 1 + 2^2}{3} = 5/3$$

$$\text{mean of } X = \frac{1 + 2}{3} = 1$$

$$(m(X))^2 = 1 = 1$$

$1 \neq 5/3$ by counterexample, $m(X^2) \neq (m(X))^2$

\sqrt{X} :

$$X = \{0, 1, 4\}$$

$$\text{mean of } \sqrt{X} = \frac{0 + 1 + 2}{3} = 1$$

$$\text{mean of } X = 5/3$$

$$\sqrt{(m(X))} = \sqrt{5/3}$$

$$1 \neq \sqrt{5/3}$$

by counterexample, $m(\sqrt{X}) \neq \sqrt{m(X)}$